\subsection*{Question 2}
We first create a morphism from \lstinline{Maybe} to \lstinline{Maybe'}:

\begin{lstlisting}
f :: Maybe a -> Maybe' a
f Nothing = Left (Const ())
f (Just x) = Right (Identity x)
\end{lstlisting}

Then we create a morphism from \lstinline{Maybe'} to \lstinline{Maybe}:

\begin{lstlisting}
f' :: Maybe' a -> Maybe a
f' (Left _) = Nothing
f' (Right (Identity x)) = Just x
\end{lstlisting}

Now we show that \lstinline{f.f' = id}. We start with the \lstinline{Left} case:

\begin{lstlisting}
(f.f') (Left (Const ())) = f (f' (Left (Const ())))
                         = f Nothing
                         = Left (Const ())
\end{lstlisting}

And now the \lstinline{Right} case:

\begin{lstlisting}
(f.f') (Right (Identity x)) = f (f' (Right (Identity x)))
                            = f (Just x)
                            = Right (Identity x)
\end{lstlisting}

Finally, we show that \lstinline{f'.f = id}. We start with the
\lstinline{Nothing} case:

\begin{lstlisting}
(f'.f) Nothing = f' (f Nothing)
               = f' (Left (Const ()))
               = Nothing
\end{lstlisting}

And now the \lstinline{Just} case:

\begin{lstlisting}
(f'.f) (Just x) = f' (f (Just x))
                = f' (Right (Identity x))
                = Just x
\end{lstlisting}
