\subsection{Question 1}

We show that \lstinline{Pair} is isomorphic to another bifunctor,
\lstinline{(,)}. Firstly, we create a morphism from \lstinline{Pair} to
\lstinline{(,)}:

\begin{lstlisting}
-- (,) a b = (a, b)
f :: Pair a b -> (a, b)
f (Pair x y) = (x, y)
\end{lstlisting}

Then we create a morphism from \lstinline{(,)} to \lstinline{Pair}:

\begin{lstlisting}
f' :: (a, b) -> Pair a b
f' (x, y) = Pair x y
\end{lstlisting}

Next, we show that \lstinline{f.f' = id}.

\begin{lstlisting}
(f.f') (x, y) = f (f' (x,y))
              = f (Pair x y)
              = (x, y)
\end{lstlisting}

And finally we show that \lstinline{f'.f = id}:

\begin{lstlisting}
(f'.f) (Pair x y) = f' (f (Pair x y))
                  = f' (x, y)
                  = Pair x y
\end{lstlisting}

We then implement the \lstinline{Bifunctor} methods for \lstinline{Pair}:

\begin{lstlisting}
instance Bifunctor Pair where
  bimap f g (Pair x y) = Pair (f x) (g y)
  first f (Pair x y) = Pair (f x) y
  second f (Pair x y) = Pair x (f y)
\end{lstlisting}

Firstly, we show that the default implementation for \lstinline{bimap} is
compatible with \lstinline{first} and \lstinline{second}:

\begin{lstlisting}
bimap f g (Pair x y) = (first f.second g) (Pair x y)
                     = first f (second g (Pair x y))
                     = first f (Pair x (g y))
                     = Pair (f x) (g y)
\end{lstlisting}

Secondly, we show that the default implementation for \lstinline{first} is
compatible with \lstinline{bimap}:

\begin{lstlisting}
first f (Pair x y) = bimap f id (Pair x y)
                   = Pair (f x) (id y)
                   = Pair (f x) y
\end{lstlisting}

Finally, we show that the default implementation for \lstinline{second} is
compatible with \lstinline{bimap}:

\begin{lstlisting}
second f (Pair x y) = bimap id f (Pair x y)
                    = Pair (id x) (f y)
                    = Pair x (f y)
\end{lstlisting}
